theories/Sem/Destroy.v
@@ -1,0 +1,14 @@
+(*
+ * Copyright (C) BedRock Systems Inc. 2019 Gregory Malecha
+ *
+ * SPDX-License-Identifier:AGPL-3.0-or-later
+ *)
+Require Import Cpp.Ast.
+From Cpp.Sem Require Import
+     Semantics Logic Wp PLogic.
+
+(* remove from the stack *)
+Definition destroy {resolve} ti (parent : Dtor_type) (cls : globname) (v : val) (Q : mpred) : mpred :=
+  Exists da, _global (dtor_name parent cls) &~ da **
+                     |> fspec (resolve:=resolve) da (v :: nil) ti
+                     (fun _ => _at (_eq v) (tany (Tref cls)) ** Q).
